rich_raven_lang/trnsl.v
@@ -52,14 +52,14 @@ Section MainTranslation.
     (* Definition stack_to_stack_frame (stk : stack) : stack_frame := 
     . *)
   
-    Definition sym_stk_eq_stk_frm (stk : stack) (stk_frm : stack_frame) : Prop :=
-      (forall (x : var) (le : LExpr), (stk !! x = Some le) -> (∃ (v : lang.val),  (stk_frm.(locals) !! x = Some v) /\ (LExpr_holds (LBinOp EqOp le (LVal (trnsl_val v)))))) /\
+    Definition sym_stk_eq_stk_frm (stk : stack) (stk_frm : stack_frame) (mp : symb_map): Prop :=
+      (forall (x : var) (lv : lvar), (stk !! x = Some lv) -> (∃ (v : lang.val),  (stk_frm.(locals) !! x = Some v) /\ (LExpr_holds (LBinOp EqOp (LVar lv) (LVal (trnsl_val v))) mp))) /\
       
-      (forall (x : var) (v : lang.val), (stk_frm.(locals) !! x = Some v) -> (∃ (le : LExpr), (stk !! x = Some le) /\ (LExpr_holds (LBinOp EqOp le (LVal (trnsl_val v)))))).
+      (forall (x : var) (v : lang.val), (stk_frm.(locals) !! x = Some v) -> (∃ (lv : lvar), (stk !! x = Some lv) /\ (LExpr_holds (LBinOp EqOp (LVar lv) (LVal (trnsl_val v))) mp))).
 
-    Lemma sym_stk_eq_stk_frm_func (stk : stack) (stk_frm1 : stack_frame) (stk_frm2 : stack_frame) :
-      sym_stk_eq_stk_frm stk stk_frm1 ->
-      sym_stk_eq_stk_frm stk stk_frm2 ->
+    Lemma sym_stk_eq_stk_frm_func (stk : stack) (stk_frm1 : stack_frame) (stk_frm2 : stack_frame) (mp : symb_map) :
+      sym_stk_eq_stk_frm stk stk_frm1 mp ->
+      sym_stk_eq_stk_frm stk stk_frm2  mp->
       stk_frm1 = stk_frm2.
     Proof.
       intros H1 H2.
@@ -80,8 +80,8 @@ Section MainTranslation.
         specialize (H2f i le Hstki).
         destruct H2f as [v' [Hstkfrm2i HLexprH2]].
         apply EqOp_refl in HLexprH.
-        pose proof (EqOp_trans _ _ _ HLexprH HLexprH2) as HE.
-        pose proof (EqpOp_LVal _ _ HE) as HE2.
+        pose proof (EqOp_trans _ _ _ _ HLexprH HLexprH2) as HE.
+        pose proof (EqpOp_LVal _ _ _ HE) as HE2.
         apply trnsl_val_inj in HE2.
         subst v'.
         simpl in Hstkfrm2i. done.
@@ -102,50 +102,71 @@ Section MainTranslation.
           * done.
     Qed.
 
+    Definition symb_stk_to_stk_frm (stk : stack) (mp : symb_map) : stack_frame :=
+      StackFrame (fmap (λ v, trnsl_lval (mp v)) stk).
 
-    Definition trnsl_hoare_triple (stk : stack) (stk_frm : stack_frame) (stk_id: stack_id) (p : assertion) (a1 : AtomicAnnotation) (cmd : stmt) (stk' : stack) (stk_frm' : stack_frame) (q : assertion) (a2 : AtomicAnnotation) : iProp rrl_lang.Σ :=
-        match (trnsl_stmt cmd stk), (trnsl_assertion p), (trnsl_assertion q) with
-        | Error, _, _ | _, None, _ | _, _, None => True
-        | None', Some p', Some q' => 
-          (p' ∗ trnsl_atomic_annotation (inv_set_to_namespace a1.1) a1) -∗ |={(inv_set_to_namespace a1.1), (inv_set_to_namespace a2.1) }=> (q' ∗ trnsl_atomic_annotation (inv_set_to_namespace a2.1) a2)
-        | Some' s, Some p', Some q' => 
-          ⌜sym_stk_eq_stk_frm stk stk_frm⌝ -∗
-          ⌜sym_stk_eq_stk_frm stk' stk_frm'⌝ -∗
-          {{{ p' ∗ stack_own[ stk_id, stk_frm ] }}}  to_rtstmt stk_id s  {{{ RET lang.LitUnit; q' ∗ stack_own[ stk_id, stk_frm' ] }}}
+    Lemma trnsl_expr_interp_lexpr_compatibility stk e lv mp : trnsl_expr_lExpr stk e = Some (LVal lv) -> expr_step e (symb_stk_to_stk_frm stk mp) (Val (trnsl_lval lv)).
+    Admitted.
+
+    Definition trnsl_hoare_triple (stk : stack) (stk_id: stack_id) (p : assertion) (a1 : AtomicAnnotation) (cmd : stmt) (stk' : stack) (q : assertion) (a2 : AtomicAnnotation) (mp : symb_map) : iProp rrl_lang.Σ :=
+        match (trnsl_stmt cmd) with 
+        | Error => True
+        | None' =>
+          match (trnsl_assertion p mp), 
+                (trnsl_assertion q mp) with
+          | None, _ | _, None => True
+          | Some p', Some q' =>
+            p' ∗ stack_own[ stk_id, symb_stk_to_stk_frm stk mp ] -∗ (q' ∗ stack_own[ stk_id, symb_stk_to_stk_frm stk' mp])
+          end
+        
+        | Some' s =>
+          match (trnsl_assertion p mp), 
+                (trnsl_assertion q mp) with
+          | None, _ | _, None => True
+          | Some p', Some q' => 
+            {{{ p' ∗ stack_own[ stk_id, symb_stk_to_stk_frm stk mp ] }}}  
+              to_rtstmt stk_id s 
+            {{{ RET lang.LitUnit; q' ∗ stack_own[ stk_id, symb_stk_to_stk_frm stk' mp] }}}
+          end
         end
     .
   
-    Theorem rrl_validity stk stk_frm stk_id p a1 cmd stk' stk_frm' q a2 :
-      RavenHoareTriple stk p a1 cmd stk' q a2 ->
-      ⊢ (trnsl_hoare_triple stk stk_frm stk_id p a1 cmd stk' stk_frm' q a2).
+    Theorem rrl_validity stk stk_id p a1 cmd stk' q a2 :
+      forall mp, RavenHoareTriple stk p a1 cmd stk' q a2 ->
+      ⊢ (trnsl_hoare_triple stk stk_id p a1 cmd stk' q a2 mp).
     Proof.
-      intros H.
-      destruct H as [ | | | | | | | | | | | | | | | | ].
+      intros mp H.
+      destruct H as 
+      [ | 
+      | stk i1 i2 mask v fld e old_val new_val lv Hatm HLexpr1 HLexpr2 
+      | | | | | | | | | | | | | | ].
       3: {
         unfold trnsl_hoare_triple.
-        destruct (trnsl_stmt (FldWr e1 fld e2) stk) eqn:Ht. 2:{done. }
+        destruct (trnsl_stmt (FldWr v fld e)) eqn:Ht. 2: done.
         { inversion Ht. } 
 
         inversion Ht. simpl. 
-        destruct (trnsl_lval old_val); destruct (trnsl_lval new_val); simpl; iIntros; try done.
+        (* destruct (trnsl_lval old_val); destruct (trnsl_lval new_val); simpl; iIntros; try done. *)
         - iIntros (Φ). iModIntro.
         iIntros "[Hstk1 Hstk2] HΦ".
 
         iDestruct "Hstk1" as "[%l [%Hlexpr1 Hlfld]]".
         
-        iApply (wp_heap_wr stk_id stk_frm _ _ _ l _ _ with "[Hstk2 Hlfld]").
+        iApply (wp_heap_wr stk_id (symb_stk_to_stk_frm stk mp) _ _ _ l _ _ with "[Hstk2 Hlfld]").
 
 
         2: {
           iModIntro. iIntros "[HstkO Hlpt]".
           iApply "HΦ". iFrame.
-          iSplitR. { iPureIntro. done. }
-          pose proof (sym_stk_eq_stk_frm_func _ _ _ H2 H4). subst stk_frm'. iFrame.
+          iPureIntro. done.
         }
         
         1: {
           iFrame.
-          admit.
+          iSplit.
+          { iPureIntro. simpl. rewrite lookup_fmap. rewrite HLexpr1. simpl. apply f_equal. rewrite Hlexpr1. simpl. apply f_equal. destruct l. simpl. done. }
+
+          { iPureIntro. apply trnsl_expr_interp_lexpr_compatibility. done. }
         }
   
     Admitted.
